new/proof/github_com/goose_lang/goose/model/channel/logatom/chan_au_send.v
@@ -12,10 +12,11 @@ Section atomic_specs.
 Context `{hG: heapGS Σ, !ffi_semantics _ _}.
 Context {sem_fn : GoSemanticsFunctions} {pre_sem : go.PreSemantics}
   {sem : go.ChanSemantics}.
-Collection W := sem_fn + pre_sem + sem.
+Collection Wp := sem_fn + pre_sem + sem.
 
 Context `[!chanG Σ V].
 Context `[!ZeroVal V] `[!TypedPointsto V] `[!IntoValTyped V t].
+Collection W := Wp + IntoValTyped0.
 
 Implicit Types (ch : loc) (γ : chan_names) (v : V).
 
